Finish rewriting TreeSet, try intersection

src/hog/TreeSet.lean
@@ -2,6 +2,7 @@ import Mathlib.Init.Algebra.Order
 import Mathlib.Tactic.LibrarySearch
 import Mathlib.Tactic.Tauto
 import Mathlib.Mathport.Syntax
+import Mathlib.Tactic.Basic
 import Mathlib.Logic.Basic
 import Init.Core
 import Init.Prelude
@@ -105,19 +106,25 @@ instance Bounded_linear_order (α : Type) [LinearOrder α] : LinearOrder (Bounde
       | apply decidable_of_iff False ; simp; by_contra; contradiction
       | apply foo'
     )
-    
 
+-- Definition of binary search tree
 inductive Stree (α : Type) [LinearOrder α] : ∀ {low high : Bounded α}, low < high → Type
   | empty : ∀ {low high} (p : low < high), Stree α p
   | leaf : ∀ {low high} (x : α) (lowx : low < element x) (xhigh : element x < high), Stree α (lt_trans lowx xhigh)
   | node : ∀ {low high} (x : α) {q : low < element x} {r : element x < high}
              (left : Stree α q) (right : Stree α r), Stree α (lt_trans q r)
 
+lemma fou : 20 < 42 := by
+  simp
 
--- example: Stree Nat (by library_search) :=
---   Stree.node 20 
---     (Stree.empty (by library_search))
---     (Stree.leaf 42 (by { sorry } : 20 < 42) (by library_search))
+lemma fuu : @LT.lt (Bounded Nat) (@Bounded_has_lt Nat Preorder.toLT) (element 20) (element 42) := by
+  have h : 20 < 42 := fou
+  assumption
+
+-- example: @Stree Nat (_) (bottom) (top) h :=
+--   Stree.node 20
+--     (Stree.empty (by rfl))
+--     (Stree.leaf 42 (fuu) (by {  }))
 
 @[reducible]
 def Stree.elem {α : Type} [LinearOrder α] (x : α) :
@@ -172,49 +179,53 @@ theorem Stree.elem_low {α : Type} [LinearOrder α] (x : α)
 
 theorem Stree.elem_high {α : Type} [LinearOrder α] (x : α)
   {low high : Bounded α} {p : low < high} (t : Stree α p) :
-  Stree.elem x t = tt → element x < high := by
-  sorry
-  -- induction t with _ _ _ A B C D E low high y I J left right ih_right ih_left,
-  -- { obviously },
-  -- { obviously },
-  -- { apply (decidable.lt_by_cases x y),
-  --   { intro xy, simp [Stree.elem, decidable.lt_by_cases, xy], intro, transitivity' y, obviously },
-  --   { intro xy, obviously },
-  --   { intro yx, simp [Stree.elem, decidable.lt_by_cases, yx, lt_asymm yx], obviously }
-  -- }
+  Stree.elem x t = true → element x < high := by
+  intro h
+  induction t with
+  | empty _ => contradiction
+  | leaf _ _ _ => 
+    simp at h
+    rw [h]
+    assumption
+  | node y l r left_ih right_ih =>
+    simp at h
+    cases h with
+    | inl hp =>
+      cases hp with
+      | inl hpp => rw [hpp]; assumption
+      | inr hpq =>
+        have h' : element x < element y := by apply left_ih hpq
+        apply lt_trans h'
+        assumption
+    | inr hq => apply right_ih hq
 
+#check lt_by_cases
 
 @[reducible]
 def Stree.insert {α : Type} [LinearOrder α] (x : α) :
   ∀ {low high : Bounded α} {p : low < high} (t : Stree α p), low < element x → element x < high → Stree α p
   | low, high, p, (Stree.empty _), lowx, xhigh => Stree.leaf x lowx xhigh
-  | low, high, p, (Stree.leaf y lowy yhigh), lowx, xhigh => sorry
-      -- Decidable.lt_by_cases x y
-      --   (fun xy => Stree.node y (Stree.leaf x lowx xy) (Stree.empty yhigh))
-      --   (fun _ => Stree.leaf y lowy yhigh)
-      --   (fun yx => Stree.node y (Stree.empty lowy) (Stree.leaf x yx xhigh))
-  | low, high, p, (Stree.node y left right), lowx, xhigh => sorry
-      -- decidable.lt_by_cases x y
-      --   (fun xy => Stree.node y (@Stree.insert _ y _ left lowx xy) right)
-      --   (fun _ => Stree.node y left right)
-      --   (fun yx => Stree.node y left (@Stree.insert y _ _ right yx xhigh))
+  | low, high, p, (Stree.leaf y lowy yhigh), lowx, xhigh =>
+    lt_by_cases x y
+      (fun xy => Stree.node y (Stree.leaf x lowx xy) (Stree.empty yhigh))
+      (fun _ => Stree.leaf y lowy yhigh)
+      (fun yx => Stree.node y (Stree.empty lowy) (Stree.leaf x yx xhigh))
+  | low, high, p, (Stree.node y left right), lowx, xhigh =>
+    lt_by_cases x y
+      (fun xy => Stree.node y (@Stree.insert _ _ x _ _ _ left lowx xy) right)
+      (fun _ => Stree.node y left right)
+      (fun yx => Stree.node y left (@Stree.insert _ _ x _ _ _ right yx xhigh))
 
-lemma elem_insert (α : Type) [LinearOrder α] (x : α) {low high : Bounded α}
-  {lowx : low < element x} {xhigh : element x < high} (t : Stree α (lt_trans lowx xhigh)) :
+theorem elem_insert (α : Type) [LinearOrder α] (x : α) {low high : Bounded α}
+  {lowx : low < element x} {xhigh : element x < high} (p : low < high) (t : Stree α p) :
   Stree.elem x (Stree.insert x t lowx xhigh) := by
-  sorry
-  -- induction t with _ _ _ _ _ y _ _ _ _ y _ _ _ _ ih_left ih_right,
-  -- { simp },
-  -- { apply (decidable.lt_by_cases x y),
-  --   { intro xy, simp [Stree.elem, Stree.insert, decidable.lt_by_cases, xy] },
-  --   { intro xy, simp [Stree.elem, Stree.insert, decidable.lt_by_cases, xy] },
-  --   { intro yx, simp [Stree.elem, Stree.insert, decidable.lt_by_cases, lt_asymm, yx] }
-  -- },
-  -- { apply (decidable.lt_by_cases x y),
-  --   { intro xy, simp [Stree.elem, Stree.insert, decidable.lt_by_cases, xy], apply ih_left },
-  --   { intro xy, simp [Stree.elem, Stree.insert, decidable.lt_by_cases, xy, lt_irrefl] },
-  --   { intro yx, simp [Stree.elem, Stree.insert, decidable.lt_by_cases, lt_asymm, yx], apply ih_right }
-  -- } 
+  induction t with
+  | empty _ => simp
+  | leaf y _ _ =>
+    apply lt_by_cases x y <;> (intro h; simp [Stree.insert, lt_by_cases, h, lt_asymm])
+  | node y l r left_ih right_ih =>
+    apply lt_by_cases x y <;> intro h <;>
+    simp [Stree.insert, lt_by_cases, h, lt_asymm, left_ih, right_ih]
 
 @[reducible]
 def Stree.forall {α : Type} [LinearOrder α] (p : α → Prop) [DecidablePred p] :
@@ -231,18 +242,28 @@ def Stree.option_forall {α : Type} [LinearOrder α] (p : α → Prop) [Decidabl
 
 lemma Stree.forall_is_forall {α : Type} [LinearOrder α] (p : α → Prop) [DecidablePred p]:
   ∀ {low high : Bounded α} {b : low < high} (t : Stree α b), 
-  Stree.forall p t = tt → ∀ (x : α), Stree.elem x t → p x :=  by
-  sorry
-  -- intros low high b t,
-  -- induction t with _ _ _ _ _ _ _ _ _ _  y,
-  -- { simp },
-  -- { simp [Stree.forall] },
-  -- { simp [Stree.forall], intros py lall rall x,
-  --   apply (decidable.lt_by_cases x y),
-  --   { intro xy, simp [ Stree.elem, decidable.lt_by_cases, xy], tautology },
-  --   { intro xy, simp [ Stree.elem, decidable.lt_by_cases, xy], assumption },
-  --   { intro yx, simp [ Stree.elem, decidable.lt_by_cases, yx, lt_asymm yx], tautology },
-  -- }
+  Stree.forall p t = true → ∀ (x : α), Stree.elem x t → p x :=  by
+  intros low high b t
+  induction t with
+  | empty _ => simp
+  | leaf y _ _ => simp
+  | node y l r left_ih right_ih =>
+    simp
+    intros py lall rall x
+    apply lt_by_cases x y <;>
+    { intro xy
+      intro h
+      cases h with
+      | inl hp =>
+        cases hp with
+        | inl hpp => rw [hpp]; exact py
+        | inr hpq =>
+          apply left_ih lall
+          exact hpq
+      | inr hq =>
+        apply right_ih rall
+        exact hq
+    }
 
 @[reducible]
 def Stree.exists {α : Type} [LinearOrder α] :
@@ -253,44 +274,77 @@ def Stree.exists {α : Type} [LinearOrder α] :
 
 lemma Stree.exists_is_exists {α : Type} [LinearOrder α] (p : α → Bool) :
   ∀ {low high : Bounded α} {b : low < high} (t : Stree α b), 
-  Stree.exists t p = tt → ∃ (x : α), Stree.elem x t ∧ p x := by
-  sorry
-  -- intros low high b t,
-  -- induction t with low high lh D E F G H I J y L M left right ih_left ih_right,
-  -- { simp [Stree.exists] },
-  -- { simp [Stree.exists] },
-  -- { simp, intro h, cases h with h1 ept,
-  --   { cases h1 with pyt ept, 
-  --     { existsi y, simp [pyt, Stree.elem, decidable.lt_by_cases] },
-  --     { obtain ⟨z, zleft, pz⟩ := ih_left ept,
-  --       existsi z,
-  --       have zy : z < y := Stree.elem_high z left zleft,
-  --       simp [Stree.elem, decidable.lt_by_cases, zy], tautology
-  --     }
-  --   },
-  --   { obtain ⟨z, zright, pz⟩ := ih_right ept,
-  --     existsi z,
-  --     have yz : y < z := Stree.elem_low z right zright,
-  --     simp [Stree.elem, decidable.lt_by_cases, yz, lt_asymm yz], tautology }
-  -- }
+  Stree.exists t p = true → ∃ (x : α), Stree.elem x t ∧ p x := by
+  intros low high b t h
+  induction t with
+  | empty _ => simp at h
+  | leaf y _ _ => simp [Stree.exists] at *; exact h
+  | node y l r left_ih right_ih =>
+    simp at h
+    cases h with
+    | inl hp =>
+      cases hp with
+      | inl hpp => apply Exists.intro y; simp [hpp]
+      | inr hpq =>
+        simp
+        obtain ⟨ x, hx ⟩ := left_ih hpq
+        apply Exists.intro x
+        simp [hx]
+    | inr hq =>
+      simp
+      obtain ⟨ x, hx ⟩ := right_ih hq
+      apply Exists.intro x
+      simp [hx]
 
--- def Stree.intersection {α : Type} [LinearOrder α] :
---   ∀ {low high : Bounded α} {b : low < high},
---   Stree α b → Stree α b → Stree α b
--- | _, _, b, (Stree.empty _), t => Stree.empty b
--- | _, _, b, t, (Stree.empty _) => Stree.empty b
--- | _, _, b, (Stree.leaf x _ _), (Stree.leaf y _ _) => if x = y then (Stree.leaf x _ _) else Stree.empty b
--- | _, _, b, (Stree.node x left right), (Stree.leaf y _ _) => 
---     if x = y then (Stree.leaf x _ _) 
---     else if Stree.elem y left then (Stree.leaf y _ _)
---     else if Stree.elem y right then (Stree.leaf y _ _)
---     else Stree.empty b
--- | _, _, b, (Stree.leaf x _ _), (Stree.node y left right) =>
---     if x = y then (Stree.leaf x _ _) 
---     else if Stree.elem x left then (Stree.leaf x _ _)
---     else if Stree.elem x right then (Stree.leaf x _ _)
---     else Stree.empty b
--- | _, _, b, (Stree.node x left right), t =>  sorry
+def Stree.coeLow {α : Type} [l : LinearOrder α] : ∀ {low high : Bounded α} {h : low < high} (b : Bounded α) (blow : b < low),
+  Stree α h → @Stree α l b high (lt_trans blow h) :=
+  fun b blow t =>
+    match t with
+    | (Stree.empty _) => Stree.empty (lt_trans blow (by assumption))
+    | (Stree.leaf x lowx highx)  => Stree.leaf x (lt_trans blow lowx) highx
+    | (@Stree.node α l _ _ x q _ left right) => Stree.node x (@Stree.coeLow α l _ (element x) q b blow left) right
+
+def Stree.coeHigh {α : Type} [l : LinearOrder α] : ∀ {low high : Bounded α} {h : low < high} (b : Bounded α) (bhigh : high < b),
+  Stree α h → @Stree α l low b (lt_trans h bhigh) :=
+  fun b bhigh t =>
+    match t with
+    | (Stree.empty _) => Stree.empty (lt_trans' bhigh (by assumption))
+    | (Stree.leaf x lowx highx)  => Stree.leaf x lowx (lt_trans highx bhigh)
+    | (@Stree.node α l _ _ x _ r left right) => Stree.node x left (@Stree.coeHigh α l (element x) _ r b bhigh right)
+
+def Stree.coe {α : Type} [l : LinearOrder α] {low high low' high' : Bounded α} (h : low < high) (h' : low' < high') (eqLow : low' = low) (eqHigh : high' = high) :
+  Stree α h → Stree α h'
+    | (Stree.empty _) => Stree.empty _
+    | (Stree.leaf x lowx highx)  => Stree.leaf x (by { rw [eqLow]; exact lowx }) (by { rw [eqHigh]; exact highx })
+    | (Stree.node x left right) => 
+      (Stree.node x 
+        (Stree.coe (_) (by { rw [eqLow]; assumption }) (eqLow) (by rfl) left)
+        (Stree.coe (_) (by { rw [eqHigh]; assumption }) (by rfl) (eqHigh) right)
+      )
+
+def Stree.intersection {α : Type} [l : LinearOrder α] :
+  ∀ {low high : Bounded α} {b : low < high},
+  Stree α b → Stree α b → Stree α b
+| _, _, b, (Stree.empty _), t => Stree.empty b
+| _, _, b, t, (Stree.empty _) => Stree.empty b
+| _, _, b, (Stree.leaf x _ _), (Stree.leaf y _ _) => 
+  if x = y then (Stree.leaf x (by assumption) (by assumption)) 
+  else Stree.empty b
+| _, _, b, (Stree.leaf x _ _), (Stree.node y left right) =>
+  if x = y then (Stree.leaf x (by assumption) (by assumption)) 
+  else if Stree.elem x left then (Stree.leaf x (by assumption) (by assumption))
+  else if Stree.elem x right then (Stree.leaf x (by assumption) (by assumption))
+  else Stree.empty b
+| _, _, b, (Stree.node x left right), (Stree.leaf y _ _) => 
+  if x = y then (Stree.leaf x (by assumption) (by assumption)) 
+  else if Stree.elem y left then (Stree.leaf y (by assumption) (by assumption))
+  else if Stree.elem y right then (Stree.leaf y (by assumption) (by assumption))
+  else Stree.empty b
+| low, high, b, (@Stree.node α l _ _ x q r left right), (@Stree.node α l _ _ x' q' r' left' right') =>
+  if H : x = x' then (Stree.node x 
+    (@intersection α l low (element x) q left (Stree.coe q' q rfl (by rw [H]) left'))
+    (@intersection α l (element x) high r right (Stree.coe r' r (by rw [H]) rfl right')))
+  else sorry
 
 def Tset (α : Type) [lo : LinearOrder α] := @Stree α lo bottom top (by rfl)
 
@@ -300,7 +354,6 @@ def Tset.option_mem {α : Type} [LinearOrder α] (x : α) : Option (Tset α) →
   | none => false
   | (some t) => Tset.mem x t
   
-
 instance Tset.has_mem {α : Type} [LinearOrder α]: Membership α (Tset α) where
   mem := fun x t => Tset.mem x t
   
@@ -310,274 +363,11 @@ instance Tset.option_has_mem {α : Type} [LinearOrder α] : Membership α (Optio
 instance Tset.has_insert {α : Type} [LinearOrder α]: Insert α (Tset α) where
   insert := fun x t => Stree.insert x t rfl rfl 
 
--- def Tset.add {α : Type} [LinearOrder α] (x : α) (t : Tset α) := Stree.insert x t (_) (_)
+def Tset.add {α : Type} [l : LinearOrder α] (x : α) (t : Tset α) := @Stree.insert α l x bottom top (by rfl) t 
 
 lemma Tset.forall_is_forall {α : Type} [LinearOrder α] (p : α → Prop) [DecidablePred p]:
-  ∀ (t : Tset α), Stree.forall p t = tt → ∀ (x : α), x ∈ t → p x :=
+  ∀ (t : Tset α), Stree.forall p t = true → ∀ (x : α), x ∈ t → p x :=
   by apply Stree.forall_is_forall
 
--- -- def Tset.intersection {α : Type} [LinearOrder α] : Tset α → Tset α → Tset α := sorry
+-- def Tset.intersection {α : Type} [LinearOrder α] : Tset α → Tset α → Tset α := sorry
 end TreeSet
-
--- import order.lexicographic
--- import data.fintype.basic
--- import tactic
--- -- Extension of an order with a new bottom and top elements. 
--- namespace tree_set
-
--- inductive Bounded (α : Type) : Type
--- | bottom : Bounded
--- | element : α -> Bounded
--- | top : Bounded
-
--- open Bounded
-
--- instance Bounded_has_coe (α : Type) : has_coe α (Bounded α) =>
---   { coe := element }
-
--- @[simp, reducible]
--- def Bounded_le {α : Type} [has_le α] : Bounded α → Bounded α → Prop
---   | bottom _ := true
---   | (element _) bottom := false
---   | (element x) (element y) := (x ≤ y)
---   | (element _) top := true
---   | top bottom := false
---   | top (element _) := false
---   | top top := true
-
--- instance Bounded_has_le (α : Type) [has_le α] : has_le (Bounded α) :=
---   { le := Bounded_le }
-
--- @[simp, reducible]
--- def Bounded_lt {α : Type} [has_lt α] : Bounded α → Bounded α → Prop
---   | bottom bottom := false
---   | bottom (element _) := true
---   | bottom top := true
---   | (element _) bottom := false
---   | (element x) (element y) := (x < y)
---   | (element _) top := true
---   | top _ := false
-
--- instance Bounded_has_lt (α : Type) [has_lt α] : has_lt (Bounded α) :=
---   { lt := Bounded_lt }
-
--- lemma Bounded_le_trans {α : Type} [preorder α] {a b c : Bounded α} :
---   Bounded_le a b → Bounded_le b c → Bounded_le a c :=
--- begin
---   cases_matching* (Bounded α) ; try { tautology },
---   apply le_trans
--- end
-
--- instance Bounded_preorder (α : Type) [preorder α] : preorder (Bounded α) :=
---   { lt := Bounded_lt,
---     le := Bounded_le,
---     le_refl := by { intro a, cases a ; trivial },
---     le_trans := by { apply Bounded_le_trans },
---     lt_iff_le_not_le := by { intros a b, cases a ; cases b ; tautology <|>  apply lt_iff_le_not_le }
---   }
-
--- instance Bounded_partial_order (α : Type) [partial_order α]: partial_order (Bounded α) :=
---   { le_antisymm :=
---       by { intros a b,  cases a ; cases b ; try { tautology },
---            intros ab ba, congr, apply (le_antisymm ab ba) },
---     .. tree_set.Bounded_preorder α }
-
--- instance Bounded_LinearOrder (α : Type) [LinearOrder α] : LinearOrder (Bounded α) :=
---   { le_total := by { intros a b, cases a ; cases b ; try { tautology }, apply le_total },
---     decidable_le := by { intros a b, cases a ; cases b ; apply_instance },
---     .. tree_set.Bounded_partial_order α
---   }
-
--- inductive Stree (α : Type) [LinearOrder α] : ∀ {low high : Bounded α}, low < high → Type
--- | empty : ∀ {low high} (p : low < high), Stree p
--- | leaf : ∀ {low high} (x : α) (lowx : low < element x) (xhigh : element x < high), Stree (lt_trans lowx xhigh)
--- | node : ∀ {low high} (x : α) {q : low < element x} {r : element x < high}
---            (left : Stree q) (right : Stree r), Stree (lt_trans q r)
-
-
--- example: Stree ℕ (by { trivial } : bottom < top) :=
---   Stree.node 20 
---     (Stree.empty true.intro)
---     (Stree.leaf 42 (by { norm_num } : 20 < 42) true.intro)
-
--- @[reducible]
--- def Stree.elem {α : Type} [LinearOrder α] (x : α) :
---     ∀ {low high : Bounded α} {p : low < high}, Stree α p → bool
--- | low high p (Stree.empty _) := ff
--- | low high p (Stree.leaf y _ _) := (x = y)
--- | low high p (Stree.node y left right) :=
---     decidable.lt_by_cases x y
---       (λ _, Stree.elem left)
---       (λ _, tt)
---       (λ _, Stree.elem right)
-
--- def Stree.size {α : Type} [LinearOrder α] : ∀ {low high : Bounded α} {p : low < high}, Stree α p → ℕ
--- | low high p (Stree.empty _) := 0
--- | low high p (Stree.leaf x _ _) := 1
--- | low high p (Stree.node x left right) := 1 + Stree.size left + Stree.size right
-
--- theorem Stree.elem_low {α : Type} [LinearOrder α] (x : α)
---   {low high : Bounded α} {p : low < high} (t : Stree α p) :
---   Stree.elem x t = tt → low < element x :=
--- begin
---   induction t with _ _ _ _ _ _ _ _ _ _ y,
---   { obviously },
---   { obviously },
---   { apply (decidable.lt_by_cases x y),
---     { intro xy, simp [Stree.elem, decidable.lt_by_cases, xy], obviously },
---     { intro xy, obviously },
---     { intro yx, simp [Stree.elem, decidable.lt_by_cases, yx, lt_asymm yx], intro, transitivity' y, obviously }
---   }
--- end
-
--- theorem Stree.elem_high {α : Type} [LinearOrder α] (x : α)
---   {low high : Bounded α} {p : low < high} (t : Stree α p) :
---   Stree.elem x t = tt → element x < high :=
--- begin
---   induction t with _ _ _ A B C D E low high y I J left right ih_right ih_left,
---   { obviously },
---   { obviously },
---   { apply (decidable.lt_by_cases x y),
---     { intro xy, simp [Stree.elem, decidable.lt_by_cases, xy], intro, transitivity' y, obviously },
---     { intro xy, obviously },
---     { intro yx, simp [Stree.elem, decidable.lt_by_cases, yx, lt_asymm yx], obviously }
---   }
--- end
-
--- @[reducible]
--- def Stree.insert {α : Type} [LinearOrder α] (x : α) :
---   ∀ {low high : Bounded α} {p : low < high} (t : Stree α p), low < element x → element x < high → Stree α p
--- | low high p (Stree.empty _) lowx xhigh := Stree.leaf x lowx xhigh
--- | low high p (Stree.leaf y lowy yhigh) lowx xhigh :=
---     decidable.lt_by_cases x y
---       (λ xy, Stree.node y (Stree.leaf x lowx xy) (Stree.empty yhigh))
---       (λ _, Stree.leaf y lowy yhigh)
---       (λ yx, Stree.node y (Stree.empty lowy) (Stree.leaf x yx xhigh))
--- | low high p (Stree.node y left right) lowx xhigh :=
---     decidable.lt_by_cases x y
---       (λ xy, Stree.node y (@Stree.insert _ y _ left lowx xy) right)
---       (λ _, Stree.node y left right)
---       (λ yx, Stree.node y left (@Stree.insert y _ _ right yx xhigh))
-
--- lemma elem_insert (α : Type) [LinearOrder α] (x : α) {low high : Bounded α}
---   {lowx : low < element x} {xhigh : element x < high} (t : Stree α (lt_trans lowx xhigh)) :
---   Stree.elem x (Stree.insert x t lowx xhigh) :=
--- begin
---   induction t with _ _ _ _ _ y _ _ _ _ y _ _ _ _ ih_left ih_right,
---   { simp },
---   { apply (decidable.lt_by_cases x y),
---     { intro xy, simp [Stree.elem, Stree.insert, decidable.lt_by_cases, xy] },
---     { intro xy, simp [Stree.elem, Stree.insert, decidable.lt_by_cases, xy] },
---     { intro yx, simp [Stree.elem, Stree.insert, decidable.lt_by_cases, lt_asymm, yx] }
---   },
---   { apply (decidable.lt_by_cases x y),
---     { intro xy, simp [Stree.elem, Stree.insert, decidable.lt_by_cases, xy], apply ih_left },
---     { intro xy, simp [Stree.elem, Stree.insert, decidable.lt_by_cases, xy, lt_irrefl] },
---     { intro yx, simp [Stree.elem, Stree.insert, decidable.lt_by_cases, lt_asymm, yx], apply ih_right }
---   } 
--- end
-
--- @[reducible]
--- def Stree.forall {α : Type} [LinearOrder α] (p : α → Prop) [DecidablePred p] :
---   ∀ {low high : Bounded α} {b : low < high} (t : Stree α b), bool
--- | _ _ _ (Stree.empty _) := tt
--- | _ _ _ (Stree.leaf x _ _):= decidable.to_bool (p x)
--- | _ _ _ (Stree.node x left right) := 
---   decidable.to_bool (p x) && Stree.forall left && Stree.forall right
-
--- def Stree.option_forall {α : Type} [LinearOrder α] (p : α → Prop) [DecidablePred p] :
---   ∀ {low high : Bounded α} {b : low < high} (t : option (Stree α b)), bool
--- | _ _ _ none := ff
--- | _ _ _ (some t) := Stree.forall p t
-
--- lemma Stree.forall_is_forall {α : Type} [LinearOrder α] (p : α → Prop) [DecidablePred p]:
---   ∀ {low high : Bounded α} {b : low < high} (t : Stree α b), 
---   Stree.forall p t = tt → ∀ (x : α), Stree.elem x t → p x :=  
--- begin
---   intros low high b t,
---   induction t with _ _ _ _ _ _ _ _ _ _  y,
---   { simp },
---   { simp [Stree.forall] },
---   { simp [Stree.forall], intros py lall rall x,
---     apply (decidable.lt_by_cases x y),
---     { intro xy, simp [ Stree.elem, decidable.lt_by_cases, xy], tautology },
---     { intro xy, simp [ Stree.elem, decidable.lt_by_cases, xy], assumption },
---     { intro yx, simp [ Stree.elem, decidable.lt_by_cases, yx, lt_asymm yx], tautology },
---   }
--- end
-
--- @[reducible]
--- def Stree.exists {α : Type} [LinearOrder α] :
---   ∀ {low high : Bounded α} {b : low < high} (t : Stree α b) (p : α → bool), bool
--- | _ _ _ (Stree.empty _) _ := ff
--- | _ _ _ (Stree.leaf x _ _) p := p x
--- | _ _ _ (Stree.node x left right) p := p x || Stree.exists left p || Stree.exists right p
-
--- lemma Stree.exists_is_exists {α : Type} [LinearOrder α] (p : α → bool) :
---   ∀ {low high : Bounded α} {b : low < high} (t : Stree α b), 
---   Stree.exists t p = tt → ∃ (x : α), Stree.elem x t ∧ p x :=  
--- begin
---   intros low high b t,
---   induction t with low high lh D E F G H I J y L M left right ih_left ih_right,
---   { simp [Stree.exists] },
---   { simp [Stree.exists] },
---   { simp, intro h, cases h with h1 ept,
---     { cases h1 with pyt ept, 
---       { existsi y, simp [pyt, Stree.elem, decidable.lt_by_cases] },
---       { obtain ⟨z, zleft, pz⟩ := ih_left ept,
---         existsi z,
---         have zy : z < y := Stree.elem_high z left zleft,
---         simp [Stree.elem, decidable.lt_by_cases, zy], tautology
---       }
---     },
---     { obtain ⟨z, zright, pz⟩ := ih_right ept,
---       existsi z,
---       have yz : y < z := Stree.elem_low z right zright,
---       simp [Stree.elem, decidable.lt_by_cases, yz, lt_asymm yz], tautology }
---   }
--- end
-
--- -- def Stree.intersection {α : Type} [LinearOrder α] :
--- --   ∀ {low high : Bounded α} {b : low < high},
--- --   Stree α b → Stree α b → Stree α b
--- -- | _ _ b (Stree.empty _) t := Stree.empty b
--- -- | _ _ b t (Stree.empty _) := Stree.empty b
--- -- | _ _ b (Stree.leaf x _ _) (Stree.leaf y _ _) := if x = y then (Stree.leaf x _ _) else Stree.empty b
--- -- | _ _ b (Stree.node x left right) (Stree.leaf y _ _) := 
--- --     if x = y then (Stree.leaf x _ _) 
--- --     else if Stree.elem y left then (Stree.leaf y _ _)
--- --     else if Stree.elem y right then (Stree.leaf y _ _)
--- --     else Stree.empty b
--- -- | _ _ b (Stree.leaf x _ _) (Stree.node y left right) :=
--- --     if x = y then (Stree.leaf x _ _) 
--- --     else if Stree.elem x left then (Stree.leaf x _ _)
--- --     else if Stree.elem x right then (Stree.leaf x _ _)
--- --     else Stree.empty b
--- -- | _ _ b (Stree.node x left right) t :=  sorry
-
--- def Tset (α : Type) [lo : LinearOrder α] := @Stree α lo bottom top true.intro
-
--- def Tset.mem {α : Type} [LinearOrder α] (x : α) (t : Tset α) := Stree.elem x t
-
--- def Tset.option_mem {α : Type} [LinearOrder α] (x : α) : option (Tset α) → bool
--- | none := ff
--- | (some t) := Tset.mem x t
-
--- instance Tset.has_mem {α : Type} [LinearOrder α]: has_mem α (Tset α) :=
---   { mem := λ x t, Tset.mem x t }
-
--- instance Tset.option_has_mem {α : Type} [LinearOrder α] : has_mem α (option (Tset α)) :=
---   { mem := λ x t, Tset.option_mem x t }
-
--- instance Tset.has_insert {α : Type} [LinearOrder α]: has_insert α (Tset α) :=
---   { insert := λ x t, Stree.insert x t true.intro true.intro }
-
--- def Tset.add {α : Type} [LinearOrder α] (x : α) (t : Tset α) := Stree.insert x t true.intro true.intro
-
--- lemma Tset.forall_is_forall {α : Type} [LinearOrder α] (p : α → Prop) [DecidablePred p]:
---   ∀ (t : Tset α), Stree.forall p t = tt → ∀ (x : α), x ∈ t → p x :=
---   by apply Stree.forall_is_forall
-
--- -- def Tset.intersection {α : Type} [LinearOrder α] : Tset α → Tset α → Tset α := sorry
-
--- end tree_set
